simp determ

leanTheories/StackComp/OpSimp.lean
@@ -1,10 +1,11 @@
 import StackComp.ScLib
+
 /-!
 # Simple Language
 - This will be the language that compiles to the simple stack language
-- it will at the very least have integer arithmetic
+- it will at the very least have integer arithmetic and assignment
 
-## Syntax via BNF
+## Syntax via BNF for arithmetic
 
 ```
 aexp := i
@@ -14,42 +15,47 @@ aexp := i
   | i / i
 ```
 
-## Semantics via Transition Relationships
+## Semantics via Transition Relationships for arithmetic
 
 ```
 
             ------------------------- (ANum)
                   ANum i ==> i
+
+
+                     st x = v
+            ------------------------- (AId)
+                   AId x ==> v
                   
 
-                    e1 ==> i1
-                    e2 ==> i2
+                    a1 ==> i1
+                    a2 ==> i2
             ------------------------- (APlus)
-              APlus e1 e2 ==> i1 + i2 
+              APlus a1 a2 ==> i1 + i2 
 
 
-                    e1 ==> i1
-                    e2 ==> i2
+                    a1 ==> i1
+                    a2 ==> i2
             ------------------------- (APlus)
-              APlus e1 e2 ==> i1 + i2 
+              APlus a1 a2 ==> i1 + i2 
 
 
-                    e1 ==> i1
-                    e2 ==> i2
+                    a1 ==> i1
+                    a2 ==> i2
             -------------------------- (AMinus)
-             AMinus e1 e2 ==> i1 - i2 
+             AMinus a1 a2 ==> i1 - i2 
 
 
-                    e1 ==> i1
-                    e2 ==> i2
+                    a1 ==> i1
+                    a2 ==> i2
             ------------------------- (AMult)
-              AMult e1 e2 ==> i1 * i2 
+              AMult a1 a2 ==> i1 * i2 
 
 
-                    e1 ==> i1
-                    e2 ==> i2
+                    a1 ==> i1
+                    a2 ==> i2
             ------------------------- (ADiv)
-              ADiv e1 e2 ==> i1 / i2 
+              ADiv a1 a2 ==> i1 / i2 
 ```
 
 ## level of embedding
@@ -66,15 +72,14 @@ aexp := i
 
 namespace StackComp
 
-inductive aexp: Type where
-  | ANum (i : Int)
-  | AId (x : String)
-  | APlus (a1 a2 : aexp)
+/-! aexp holds the types of expressions that interact with ints -/
+inductive aexp : Type where
+  | ANum   (i : Int)
+  | AId    (x : String)
+  | APlus  (a1 a2 : aexp)
   | AMinus (a1 a2 : aexp)
-  | AMult (a1 a2 : aexp)
-  | ADiv (a1 a2 : aexp)
-
--- def aeval ()
+  | AMult  (a1 a2 : aexp)
+  | ADiv   (a1 a2 : aexp)
 
 /-!
 # Defining how arithmetic is evaluated with a Relation
@@ -84,30 +89,120 @@ inductive aexp: Type where
 - this added flexibilility in this case is not needed and only adds some complexity
 - I am showing it as a case study and possible second route for defining Simp
 -/
-inductive aevalR: aexp -> Int -> Prop :=
-  | E_ANum (i : Int) : aevalR (.ANum i) i
-  | E_APlus (e1 e2 : aexp) :
-    (aevalR e1 i1) →
-    (aevalR e2 i2) →
-    aevalR (.APlus e1 e2) (i1 + i2)
-  | E_AMinus (e1 e2 : aexp) :
-    (aevalR e1 i1) →
-    (aevalR e2 i2) →
-    aevalR (.AMinus e1 e2) (i1 - i2)
-  | E_AMult (e1 e2 : aexp) :
-    (aevalR e1 i1) →
-    (aevalR e2 i2) →
-    aevalR (.AMult e1 e2) (i1 * i2)
-  | E_ADiv (e1 e2 : aexp) :
-    (aevalR e1 i1) →
-    (aevalR e2 i2) →
-    aevalR (.ADiv e1 e2) (i1 / i2)
+inductive aevalR: aexp → state → Int → Prop :=
+  | E_ANum  (i : Int) (st : state): aevalR (.ANum i) st i
+  | E_AId   (x : String) (st : state): aevalR (.AId x) st (st x)
+  | E_APlus (a1 a2 : aexp) (st : state):
+    (aevalR a1 st i1) →
+    (aevalR a2 st i2) →
+    aevalR (.APlus a1 a2) st (i1 + i2)
+  | E_AMinus (a1 a2 : aexp) (st : state):
+    (aevalR a1 st i1) →
+    (aevalR a2 st i2) →
+    aevalR (.AMinus a1 a2) st (i1 - i2)
+  | E_AMult (a1 a2 : aexp) (st : state):
+    (aevalR a1 st i1) →
+    (aevalR a2 st i2) →
+    aevalR (.AMult a1 a2) st (i1 * i2)
+  | E_ADiv (a1 a2 : aexp) (st : state):
+    (aevalR a1 st i1) →
+    (aevalR a2 st i2) →
+    aevalR (.ADiv a1 a2) st (i1 / i2)
 
 theorem aevalR_ex1:
-  aevalR (aexp.AMult (aexp.ANum 10) (aexp.ANum 5)) (10 * 5) :=
+  aevalR (aexp.AMult (aexp.ANum 10) (aexp.ANum 5)) empty_state (10 * 5) :=
   by
     apply aevalR.E_AMult
     { apply aevalR.E_ANum }
     { apply aevalR.E_ANum }
+
+/-! 
+# Defining how arithmetic is evaluated with a function
+- the benefits of this is we have determinism by virtue of aevel being a function
+- we have a cleaner syntax for showing examples of evaluation
+-/
+def aeval (st : state) (a : aexp) : Int :=
+  match a with
+  | .ANum i       => i
+  | .AId x        => st x
+  | .APlus a1 a2  => (aeval st a1) + (aeval st a2)
+  | .AMinus a1 a2 => (aeval st a1) - (aeval st a2)
+  | .AMult a1 a2  => (aeval st a1) * (aeval st a2)
+  | .ADiv a1 a2   => (aeval st a1) / (aeval st a2)
+
+/-!
+## Examples of evaluation
+- simple arithmetic
+- getting values from state
+-/
+#eval aeval empty_state (.APlus (.ANum 5) (.ANum 5))
+#eval aeval (empty_state["x" !-> 11]) (.AMult (.AId "x") (.ANum 5))
+
+/-! 
+# Defining rules for big step evaluation of SIMP
+- to define evaluation we will use an *inductive* definition to describe how different
+  commands `com` are evaluated.
+
+## BNF for SIMP
+
+- we have two types of primitive commands
+  - assignment, denoted with `:=`
+  - sequencing, denoted with `;`
+
+```
+com := x := a
+  | c ; c
+```
+
+## Semantics of SIMP
+
+```
+                   aeval st a = n
+            ---------------------------- (C_Asgn)
+             st =[x := a]=> st[x !-> n]
+
+
+                   st =[c1]=> st'
+                  st' =[c1]=> st''
+            ------------------------- (C_Seq)
+                st =[c1 ; c2]=> st''
+```
+-/
+
+/-! Defining the semantics of SIMP -/
+inductive com : Type where
+  | CAsgn (x : String) (a : aexp)
+  | CSeq  (c1 c2 : com)
+
+/-! Defining the Semantics of SIMP -/
+inductive ceval : com → state → state → Prop where
+  | C_Asgn : ∀ st a i x,
+    aeval st a = i → ceval (.CAsgn x a) st (st[x !-> i])
+  | C_Seq : ∀ c1 c2 st st' st'',
+    ceval c1 st st' → ceval c2 st' st'' →
+    ceval (.CSeq c1 c2) st st''
+
+/-! Proving that evaluation of SIMP is determinism -/
+theorem ceval_determ {c st st1 st2}
+  (hl : ceval c st st1)
+  (hr : ceval c st st2):
+  st1 = st2 :=
+  by induction hl generalizing st2 with
+  | C_Asgn st' a i x ha =>
+    cases hr
+    case C_Asgn i' ha' =>
+      have hi: i = i' := by
+        rw [←ha, ←ha']
+      subst hi
+      rfl
+  | C_Seq c1 c2 st' st1' st2' _ec1 _ec2 hc hc' =>
+    cases hr 
+    case C_Seq st'' hc1 hc1' =>
+      have h1 : st1' = st'' := by
+        apply hc
+        exact hc1
+      apply hc'
+      rw [h1]
+      exact hc1'
 
 end StackComp
