leanTheories/StackComp/Comp.lean
@@ -1,0 +1,7 @@
+import StackComp.OpSimp
+import StackComp.OpStack
+import StackComp.ScLib
+
+namespace StackComp
+
+end StackComp
