leanTheories/StackComp/ScLib.lean
@@ -1,13 +1,27 @@
 namespace StackComp
 
+/-! 
+# State
+- for both SIMP and Stack state is defined as a function from a string to an int
+  - in essence this is a **total map**
+  - we map strings to integer values
+- we explicitly define `state` and `empty_state`
+- we create custom notation for updating the *state map*
+  - `∀ (st : state) (v : String) (x : Int), st[v !-> x]`
+-/
+
+/-! Define state -/
 def state : Type :=
   String → Int
 
+/-! Define emtpy state -/
 def empty_state : state := λ _ => 0
 
+/-! Provide a mechanism to update state -/
 def state.update (x : String) (v : Int) (s : state) : state :=
   λ x' => if x' = x then v else s x'
 
+/-! Create custom notation for updating state -/
 macro s:term "[" x:term "!->" v:term "]" : term =>
   `(state.update $x $v $s)
 
